

6.1)

$$m(a+bX) = \frac{1}{n} \sum_{i=1}^n x_i$$

$$m(a+bX) = \frac{1}{n} \sum_{i=1}^n (a + bx_i)$$

$$m(a+bX) = \frac{1}{n} \left( \sum_{i=1}^n a + b \sum_{i=1}^n x_i \right)$$

$$m(a+bX) = \frac{1}{n} \left( Na + b \sum_{i=1}^n x_i \right)$$

$$m(a+bX) = \frac{Na}{n} + b \frac{1}{n} \sum_{i=1}^n x_i$$

$$m(a+bX) = a + b \times m(X)$$

6.2)

$$\text{cov}(X, X) = \frac{1}{n} \sum_{i=1}^n (x_i - m(X))(x_i - m(X))$$

$$\text{cov}(X, X) = \frac{1}{n} \sum_{i=1}^n (x_i - m(X))^2$$

$$\text{cov}(X, X) = s^2$$

6.3)

$$A = a + bY$$

$$a_i = a + by_i$$

$$m(A) = a + b \times m(Y)$$

$$a_i - m(A) = (a + by_i) - (a + b \times m(Y))$$

$$a_i - m(A) = b(y_i - m(Y))$$

$$\text{cov}(X, A) = \frac{1}{n} \sum_{i=1}^n (x_i - m(X)) \times b(y_i - m(Y))$$

6.3)

$$\text{Cov}(X, Y) = b \left( \frac{1}{N} \sum_{i=1}^N (x_i - m(X))(y_i - m(Y)) \right)$$

$$\text{Cov}(X, a + bY) = b \times \text{Cov}(X, Y)$$

6.4)

$$\text{Cov}(a + bX, a + bY) = b \times \text{Cov}(a + bX, Y)$$

$$\text{Cov}(a + bX, Y) = b (\text{Cov}(X, Y))$$

$$\text{Cov}(a + bX, a + bY) = b^2 \text{Cov}(X, Y)$$

6.5)

Yes, it's true because the order of the data is unaffected.

No, it's false because  $a$  shouldn't be included in  $a + b \times \text{IQR}(X)$  because it doesn't affect outcome.

$$6.6)$$

$$X = \{0.6\}$$

$$\text{Mean} = 3$$

$$(m(X))^2 = 9$$

$$X^2 = \{0.36\}$$

$$\text{Mean} = 18$$

$$\text{Mean } X^2 (18) \neq (m(X))^2 (9)$$

$$X = \{0.8\}$$

$$\text{Mean} = 4$$

$$\sqrt{m(X)} = 2$$

$$\sqrt{X} = \{0.2, 43\}$$

$$\text{Mean} = 1.42$$

$$\text{Mean } \sqrt{X} (1.42) \neq \sqrt{m(X)} (2)$$